+RestorePlanner
Signed-off-by: Alexander Diemand <codieplusplus@apax.net>

bin/lxr_assembly.ml
@@ -1,0 +1,38 @@
+(* open Lwt *)
+
+(* open Elykseer__Lxr *)
+open Elykseer__Lxr.Assembly
+(* open Elykseer__Lxr.Block *)
+open Elykseer__Lxr.Environment
+
+open Elykseer_utils
+
+let arg_verbose = ref false
+let arg_fctrl = ref ""
+let arg_aid = ref ""
+
+let argspec =
+  [
+    ("-v", Arg.Set arg_verbose, "verbose output");
+    ("-a", Arg.Set_string arg_aid, "id of assembly");
+    ("-f", Arg.Set_string arg_fctrl, "control file for LXR encoder");
+  ]
+
+let anon_args_fun _fn = ()
+
+let assembly_check e p_aid : assembly option Lwt.t =
+    Lwt.return @@ List.find_opt (fun a -> aid a = p_aid) e.assemblies
+
+(* main *)
+let main () = Arg.parse argspec anon_args_fun "lxr_assemlby: vaf";
+    let _setup = setup_environment in
+    let e = Envutils.envrestore !arg_fctrl in
+    let%lwt () = Lwt_io.printl (Utils.e2s e) in
+    let%lwt a = assembly_check e !arg_aid in
+    match a with
+    | None -> Lwt_io.printl "nothing found"
+    | Some a0 ->
+        let a1 = restore (e.config) a0 in
+        Lwt_io.printl (Utils.as2s a1)
+
+let () = Lwt_main.run (main ())
