elykseer-base/chunk.mli
@@ -1,0 +1,9 @@
+
+type t = Mlcpp_cstdio.Cstdio.File.Buffer.ta
+
+val load_from_path : string -> t option
+(* val store_to_path : t -> string *)
+
+val get : t -> int -> char
+val set : t -> int -> char -> unit
+val size : t -> int
