elykseer-base/hashing.ml
@@ -1,0 +1,2 @@
+
+let sha256 s = Sha256.to_hex @@ Sha256.string s
