theories/Buffer.v
@@ -19,17 +19,26 @@ Require Import ZArith NArith.
 (* Open Scope positive_scope. *)
 Open Scope N_scope.
 
+From LXR Require Import Conversion.
+
+
+Axiom buffer_t : Type.
+Axiom buffer_create : N -> buffer_t.
+Axiom buffer_len : buffer_t -> N.
+
 Record buffer : Type := mkbuffer
-    { width : N
-    ; height : N
+    { len : N
+    ; buf : buffer_t
     }.
-Definition new_buffer (w h : N) : buffer :=
-    {| width := w; height := h |}.
+Definition new_buffer (len : N) : buffer :=
+    {| len := len; buf := buffer_create len |}.
+Definition init_buffer (buf : buffer_t) : buffer :=
+    {| len := buffer_len buf; buf := buf |}.
 
 Definition set (b : buffer) (idx : N) (v : Z) : Prop :=
-    idx < (width b) * (height b).
+    idx < (len b).
 
 Definition get (b : buffer) (idx : N) : Prop :=
-    idx < (width b) * (height b).
+    idx < (len b).
 
 End Buffer.
